hinduction: fully support indices. find parameters and indices of induction principle without using elaborator.

src/hott/init/meta/induction.lean
@@ -94,13 +94,17 @@ end option
 
 namespace tactic
 
-open environment lean.parser expr pexpr
+open environment lean.parser expr pexpr sum
 
 variable {elab : bool}
 
-/- this doesn't work -/
--- meta def check_consistency : tactic unit :=
--- do r ← result, type_check r
+declare_trace hinduction
+private meta def mtac (t : tactic unit) : tactic unit := 
+when_tracing `hinduction t
+private meta def mtrace (msg : format) : tactic unit := 
+mtac $ trace msg
+private meta def mfail {α : Type _} (msg : format) : tactic α := 
+mtrace msg >> fail msg
 
 structure induction_info :=
   (nargs : ℕ) /- the number of arguments of the recursor -/
@@ -111,16 +115,17 @@ structure induction_info :=
   (major_premise : ℕ)
   (target : name) /- the head of the major premise -/
   (dependent : bool) /- whether the major premise occurs in the conclusion -/
-  (indices : list ℕ) /- The indices are the variables to which the motive is applied in the conclusion, other than the major premise -/
+  (indices : list ℕ) /- The indices are the variables to which the motive is applied in the conclusion, excluding the major premise -/
   (indices_in_major_premise : list ℕ) /- Position where the indices occur in the type of the major premise.
     If a index occurs more than once, then only the first occurrence is recorded.
     In this case, when applying the recursor, we don't check that the same variable occurs in these places,
     if that is not the case, we might get a confusing error message -/
+  (params : list ℕ)  /- the parameters are the other arguments of the induction principle -/
+  (params_in_major_premise : list ℕ) /- Position where the parameters occurs in the type of the major premise. See remarks from indices -/
 
 -- meta instance : has_to_format induction_info :=
 -- ⟨λH, to_fmt "#args: " ++ to_fmt H.nargs ++ "; pos. motive:  " ++ H.motive ++ "; and more."⟩
 
-/- To do: allow hinduction 1 and maybe hinduction to a variable yet to be intro'd -/
 meta def get_induction_info (nm : name) : tactic expr :=
 do let info_name := mk_str_name nm "_ind_info",
 env ← get_env,
@@ -148,117 +153,124 @@ let l₂ := l₁.gen_position $ λn' oe' es,
 tmaj ← args.nth maj_prem,
 const tgt _ ← return $ get_app_fn tmaj | fail $ to_fmt "Invalid type of major premise (at position " ++ to_fmt (maj_prem+1) ++
   "). The head is not a constant or definition.",
-if min_prem.any $ λk, to_bool (k > maj_prem) && (args.nth k).iget.has_var_idx (k - maj_prem - 1)
-  then fail $ to_fmt "Some minor premises depend on major premise. Minor premises: " ++ to_fmt (min_prem.map (+1)) ++
-    ", major premise: " ++ to_fmt (maj_prem+1)
-  else skip,
+when (min_prem.any $ λk, to_bool (k > maj_prem) && (args.nth k).iget.has_var_idx (k - maj_prem - 1)) $
+  fail $ to_fmt "Some minor premises depend on major premise. Minor premises: " ++ to_fmt (min_prem.map (+1)) ++
+    ", major premise: " ++ to_fmt (maj_prem+1),
 let dep := c.has_var_idx (len_args - maj_prem - 1),
 let mot_args := get_app_args c,
 indices_or_maj_prem ← mot_args.mmap (λe, do var ve ← return e | fail "Motive is applied to arguments which are not variables.",
   return $ len_args - ve - 1),
-maj_prem_args ← return $ get_app_args tmaj,
-maj_prem_arg_vars ← maj_prem_args.mmap (λe, try_core $ do var ve ← return e, return ve),
+maj_prem_arg_vars ← (get_app_args tmaj).mmap (λe, try_core $ do var ve ← head_eta e, return ve),
+mtrace $ to_fmt maj_prem_arg_vars,
 let indices := if dep then indices_or_maj_prem.init else indices_or_maj_prem,
 indices_in_major_premise ← indices.mmap (λn, do
   let l := maj_prem_arg_vars.position $ λpos var, to_bool $ var = some (maj_prem - n - 1),
-  mpos::_ ← return l | fail $ to_fmt "The index at position " ++ to_fmt (n+1) ++ " is not an argument of " ++ to_fmt tgt,
+  mpos::_ ← return l | fail $ to_fmt "The index at position " ++ to_fmt (n+1) ++ " is not an argument of the major premise.",
+  return $ mpos),
+let params := (list.range len_args).filter $ λk, k ≠ motive ∧ k ≠ maj_prem ∧ ¬pre_min_prem.mem k ∧ ¬indices.mem k,
+params_in_major_premise ← params.mmap (λn, do
+  let l := maj_prem_arg_vars.position $ λpos var, to_bool $ var = some (maj_prem - n - 1),
+  mpos::_ ← return l | fail $ to_fmt "The parameter at position " ++ to_fmt (n+1) ++ " is not an argument of the major premise.",
   return $ mpos),
 let e := `(induction_info.mk %%(reflect len_args) %%(reflect motive) %%(reflect min_prem) %%(reflect min_prem_arity)
-  %%(reflect type_class_prem) %%(reflect maj_prem) %%(reflect tgt) %%(reflect dep) %%(reflect indices) %%(reflect indices_in_major_premise)),
+  %%(reflect type_class_prem) %%(reflect maj_prem) %%(reflect tgt) %%(reflect dep) %%(reflect indices) %%(reflect indices_in_major_premise) %%(reflect params) %%(reflect params_in_major_premise)),
 add_decl $ mk_definition info_name [] `(induction_info) e,
 return e
-
-declare_trace hinduction
-private meta def mtrace (msg : format) : tactic unit :=
-when_tracing `hinduction $ trace msg
-private meta def mfail {α : Type _} (msg : format) : tactic α :=
-mtrace msg >> fail msg
 
 @[user_attribute] meta def induction_attribute : user_attribute :=
 { name      := `induction,
   descr     := "HoTT attribute for induction principles",
-  after_set := some $ λ n _ _, get_induction_info n >> return () }
+  after_set := some $ λ n _ _, get_induction_info n >> skip }
 
 meta def get_rec_info (nm : name) : expr :=
 expr.const (mk_str_name nm "_ind_info") []
 
--- meta def pexpr_bind_lambda (e : expr) : expr → pexpr
--- | (local_const n pp_n bi _) := lam pp_n bi mk_placeholder $ to_pexpr $ e.abstract_local n
--- | _                         := to_pexpr e
-
 /- TODO: [later] add support for let-expressions (in revert_kdeps) -/
-meta def hinduction_core (h : expr) (rec : name) (ns : list name) (info : expr) : tactic unit :=
-focus1 $ do
-nargs ← eval_expr ℕ `(induction_info.nargs %%info),
-maj_prem_pos ← eval_expr ℕ `(induction_info.major_premise %%info),
-motive_pos ← eval_expr ℕ `(induction_info.motive %%info),
-mp_ar ← eval_expr (list ℕ) `(induction_info.minor_premise_arity %%info),
---indices ← eval_expr (list ℕ) `(induction_info.indices %%info),
-index_pos ← eval_expr (list ℕ) `(induction_info.indices_in_major_premise %%info),
-th ← infer_type h,
-let th_args := get_app_args th,
-(indices, reverts) ← list.unzip.{0 0} <$> (index_pos.mmap $ λk, (do
-  let e := (th_args.nth k).iget,
-  local_const _ _ _ _ ← return e | mfail "Invalid recursor application with indices. There is an index which doesn't occur as variable in the type of major premise.",
-  revs ← kdependencies e,
-  k ← revert_lst $ revs.filter (≠ h),
-  return (e, k))),
+/- t is the type of h, possiby unfolded -/
+meta def hinduction_core (h t : expr) (rec : name) (ns : list name) (info : expr) : tactic unit :=
+focus1 $ do 
+induction_info.mk nargs motive_pos _/-minor_premise position-/ mp_ar _/-type class premises-/ maj_prem_pos
+  _/-target-/ dep index_pos index_pos_maj params_pos params_pos_maj ← eval_expr induction_info info,
+let t_args := get_app_args t,
+indices : list expr ← index_pos_maj.mmap $ λk, (do 
+  e ← whnf (t_args.nth k).iget,
+  local_const _ _ _ _ ← return e | pp e >>= λmsg, mfail (to_fmt "Invalid recursor application with indices. There is an index which doesn't occur as variable in the type of major premise.\nSolution: generalize expression\n" ++ msg),
+  return e),
+mtrace $ to_fmt "indices: " ++ to_fmt indices,
+let params : list expr := params_pos_maj.map $ λk, (t_args.nth k).iget,
+reverts : list ℕ ← indices.mmap $ λe, (do
+  revs ← kdependencies e, 
+  revert_lst $ revs.filter (λx, x ≠ h ∧ ¬indices.mem x)),
 t ← target,
 crec ← mk_explicit <$> to_pexpr <$> mk_const rec,
--- let mot := to_pexpr $ indices.reverse.foldl bind_lambda t,
--- trace mot,
-let flist : list pexpr := ((list.repeat mk_placeholder nargs).replace_position maj_prem_pos (to_pexpr h)).replace_position motive_pos mk_placeholder,
-let fapp : pexpr := flist.foldl app crec,
--- trace fapp,
-efapp ← (to_expr ``(%%fapp : %%t) tt).do_on_failure $
-  λmsg, let msg' : format := "Induction tactic failed. Recursor is not applicable.\n" ++ msg in mtrace msg' >> return msg',
--- trace "foo",
+let indices_plus := if dep then indices.append [h] else indices,
+mot ← bind_lambdas indices_plus t,
+-- let mot := mk_placeholder,
+pp t >>= λm, mtrace $ to_fmt "target: " ++ m,
+pp mot >>= λm, mtrace $ to_fmt "motive: " ++ m,
+let mot' := to_pexpr mot,
+/- a list with placeholders, with the major premise and motive filled in-/
+let flist : list pexpr := ((list.repeat mk_placeholder nargs).replace_position maj_prem_pos (to_pexpr h)).replace_position motive_pos mot',
+/- also fill in the indices -/
+let flist₂ : list pexpr := (list.zip index_pos indices).foldl (λe ⟨n, e'⟩, e.replace_position n $ to_pexpr e') flist,
+/- also fill in the parameters -/
+let flist₃ : list pexpr := (list.zip params_pos params).foldl (λe ⟨n, e'⟩, e.replace_position n $ to_pexpr e') flist,
+mtrace $ to_fmt "List of arguments: " ++ to_fmt flist₃,
+let fapp : pexpr := flist₃.foldl app crec,
+-- mtrace $ to_fmt "Raw format of the application: " ++ to_raw_fmt fapp,
+efapp ← (to_expr ``(%%fapp : %%t)).do_on_failure $
+  λmsg, (let msg' : format := "Induction tactic failed. Recursor is not applicable.\n" ++ msg in 
+    mtrace msg' >> return msg'),
 type_check efapp <|> mfail (to_fmt "Incorrect recursor application.\nRecursors with indices are not yet supported.\n" ++ to_fmt efapp),
+mtrace $ to_fmt "Elaborated application: " ++ to_fmt efapp,
+-- mtac trace_state,
 exact efapp,
-/- to do[indices]: clear indices -/
-(all_goals $ clear h) <|> mfail "Couldn't clear major premise from context after applying the induction principle.\nPossible solution: generalize all let-expressions where the major premise occurs.",
-(all_goals $ indices.mmap' clear) <|> mfail "Couldn't clear indices from context after applying the induction principle.",
-reverts.mmap' intron,
+(all_goals $ clear h) <|> mfail ("Couldn't clear major premise from context after applying the induction principle.\n" ++ "Possible solution: generalize all let-expressions where the major premise occurs."),
+-- mtac trace_state,
+(all_goals $ indices.reverse.mmap' clear) <|> mfail "Couldn't clear indices from context after applying the induction principle.",
+reverts.mmap' intron, -- to do: only do this if minor premise has conclusion motive
 ng ← num_goals,
 guard (mp_ar.length = ng) <|> mfail "Unreachable(?) code: wrong number of minor premises",
 let names := ns.splits_pad `_ mp_ar,
-focus $ names.map $ λnms, intro_lst nms >> return ()
+focus $ names.map $ λnms, intro_lst nms >> skip
 
-meta def hinduction_using (h : expr) (nm : name) (ns' : list name) : tactic unit :=
-do t ← infer_type h,
-const ht _ ← return $ get_app_fn t | mfail $ to_fmt "Invalid major premise " ++ to_fmt h ++ ". The head of its type is not a constant or definition.",
-dept ← target >>= λtgt, kdepends_on tgt h,
-rec_info ← get_induction_info nm,
+
+/- t is the type of h, possiby unfolded, ht is the head of t, dept is whether the target depends on h -/
+meta def hinduction_using (h t : expr) (ht : name) (dept : bool) (nm : name) (ns' : list name) : tactic (unit ⊕ option (unit → format)) :=
+do rec_info ← get_induction_info nm <|> mfail (to_fmt "Invalid recursor " ++ to_fmt nm),
 tgt ← eval_expr name $ expr.app `(induction_info.target) rec_info,
 is_dept_rec ← eval_expr bool $ expr.app `(induction_info.dependent) rec_info,
-guard $ tgt = ht,
-if dept && bnot is_dept_rec then mfail $ to_fmt "Invalid recursor. " ++ to_fmt nm ++ " is not recursive" else hinduction_core h nm ns' rec_info
+guard (tgt = ht) <|> mfail (to_fmt "Recursor " ++ to_fmt nm ++ 
+  " is not applicable. The head of the induction variable is " ++ to_fmt ht ++ 
+  ", but the target of the induction principle is " ++ to_fmt tgt),
+if bnot dept || is_dept_rec then skip else mfail (to_fmt "Invalid recursor. " ++ to_fmt nm ++ " is not recursive"), 
+try_core_msg $ hinduction_core h t nm ns' rec_info
 
-meta def hinduction (h : expr) (rec : option name) (ns' : list name) : tactic unit :=
+/- t is the type of h, possiby unfolded -/
+meta def hinduction (h t : expr) (rec : option name) (ns' : list name) : tactic unit :=
+do const ht _ ← return $ get_app_fn t | mfail $ to_fmt "Invalid major premise " ++ to_fmt h ++ ". The head of its type is not a constant or definition.",
+dept ← target >>= λtgt, kdepends_on tgt h,
 match rec with
-| (some nm) := hinduction_using h nm ns'
-| none        := do
-  t ← infer_type h,
-  const ht _ ← return $ get_app_fn t | fail $ to_fmt "Invalid major premise " ++ to_fmt h ++ ". The head of its type is not a constant or definition.",
-  dept ← target >>= λtgt, kdepends_on tgt h,
-  ns ← attribute.get_instances `induction, -- to do: use rb_map to filter induction principles more quickly!?
+| some nm := extract $ hinduction_using h t ht dept nm ns'
+| none    := do
+  ns₂ ← attribute.get_instances `induction, -- to do: use rb_map to filter induction principles more quickly!?
+  let hrec := mk_str_name ht "rec",
   env ← get_env,
-  (ns.mfirst $ λnm, do { mtrace $ to_fmt "Trying " ++ to_fmt nm,
-    let info := get_rec_info nm,
-    tgt ← eval_expr name `(induction_info.target %%info),
-    guard (tgt = ht) <|> mfail "Wrong major premise.",
-    is_dept_rec ← eval_expr bool `(induction_info.dependent %%info),
-    guard (bnot dept || is_dept_rec) <|> mfail "Recursor is not dependent.",
-    hinduction_core h nm ns' info }) <|>
-  (let hrec := mk_str_name ht "rec" in
-    if env.contains $ hrec then mtrace (to_fmt "Trying default rec " ++ to_fmt hrec) >> hinduction_using h hrec ns'
-    else mfail $ to_fmt hrec ++ " doesn't exist.") <|>
-  fail "No induction principle found for this major premise."
+  ns ← if env.contains hrec
+       then (has_attribute `induction hrec >> return ns₂) <|> return (ns₂ ++ [hrec])
+       else return ns₂,
+  ns.mfirst_msg $ λnm, mtrace (to_fmt "Trying " ++ to_fmt nm) >> hinduction_using h t ht dept nm ns'
 end
 
+/-- tries to apply hinduction, but if it fails, applies whnf to the type of h and tries again -/
+meta def hinduction_whnf (h : expr) (rec : option name) (ns' : list name) : tactic unit :=
+do t ← infer_type h,
+(hinduction h t rec ns').orelse_plus $ 
+do t' ← whnf t, if t = t' then return none 
+else mtrace "Applying whnf to major premsie" >> some <$> hinduction h t' rec ns'
+
 meta def hinduction_or_induction (h : expr) (rec : option name) (ns : list name) : tactic unit :=
-induction' h ns rec -- >> (check_consistency <|> trace "normal induction failed" >> failed)
-<|> hinduction h rec ns
+hinduction_whnf h rec ns <|> induction' h ns rec
 
 /- If h is a local constant, reverts all local constants which have h in their type.
    Otherwise, generalizes h to local constant h' and adds equality H : h' = h, where H is the head of ns (if non-empty).
@@ -275,7 +287,7 @@ match h with
   do x ← mk_fresh_name, /- to do: let the user decide whether to use ginduction or induction here -/
   let (nm, nms) := (match ns with
   | []        := (`_h, [])
-  | (nm :: nms) := (nm, nms)
+  | nm :: nms := (nm, nms)
   end : name × list name),
   hgeneralize (some nm) (to_pexpr h) x,
   t ← get_local x,
@@ -291,6 +303,9 @@ open expr interactive.types lean.parser tactic interactive
 local postfix `?`:9001 := optional
 local postfix *:9001 := many
 
+/- To do: allow hinduction 1 and maybe hinduction to a variable yet to be intro'd -/
+/- to do: eta-reduce (and maybe more reductions) to variables, so that `(λx, B x)` is recognized as parameter `B` -/
+
 /-- Applies induction to p. Works also for HoTT-induction principles which may not eliminate into Prop.
     First tries the usual induction principle, and if that fails (or produces a type incorrect result)
     tries the new induction principle, which relaxes many conditions of the usual induction principle.
@@ -300,16 +315,16 @@ meta def hinduction (p : parse texpr) (rec_name : parse using_ident) (ids : pars
 focus1 $ do e ← i_to_expr p,
 rec : option name ← rec_name.mmap resolve_constant,
 n ← mmap tactic.get_local (revert.get_or_else []) >>= revert_lst,
-ind_generalize e ids $ λe' ns', tactic.hinduction_or_induction e' rec ns',
+ind_generalize e ids $ λe' ns', tactic.hinduction_whnf e' rec ns',
 all_goals $ intron n
 
 /-- Similar to hinduction, but doesn't try the usual induction principle first -/
-meta def hinduction_only (p : parse texpr) (rec_name : parse using_ident) (ids : parse with_ident_list)
+meta def hinduction_plus (p : parse texpr) (rec_name : parse using_ident) (ids : parse with_ident_list)
   (revert : parse $ (tk "generalizing" *> ident*)?) : tactic unit :=
 focus1 $ do e ← i_to_expr p,
 rec : option name ← rec_name.mmap resolve_constant,
 n ← mmap tactic.get_local (revert.get_or_else []) >>= revert_lst,
-ind_generalize e ids $ λe' ns', tactic.hinduction e' rec ns',
+ind_generalize e ids $ λe' ns', tactic.hinduction_or_induction e' rec ns',
 all_goals $ intron n
 
 end interactive
