src/hott/init/meta/basic_tactics.lean
@@ -6,24 +6,14 @@ Authors: Floris van Doorn
 import ..path0
 
 universes u v w
-namespace list
-open tactic
-meta def mmap_filter {α : Type u} {β : Type v} (f : α → tactic (option β)) : list α → tactic (list β)
-| []       := return []
-| (x :: xs) := do oy ← f x, ys ← mmap_filter xs, some y ← return oy | return ys, return $ y :: ys
 
-end list
-namespace option
+namespace name
 
-/-- The mmap for options. -/
-def mmap {m : Type u → Type v} [monad m] {α : Type w} {β : Type u} (f : α → m β) : option α → m (option β)
-| none     := return none
-| (some x) := do y ← f x, return $ some y
+meta def append_postfix : name → string → name
+| (mk_string s p) s' := mk_string (s ++ s') p
+| x               s' := x
 
-def iget {α : Type u} [inhabited α] : option α → α
-| none     := default α
-| (some x) := x
-end option
+end name
 
 namespace expr
 
@@ -36,21 +26,71 @@ meta def destruct_pis : expr elab → list name × list binder_info × list (exp
 instance inhabited_binder_info : inhabited binder_info :=
 ⟨binder_info.default⟩
 
-end expr
+open pexpr
+meta def to_raw_pexpr : expr → pexpr
+| (var n)                     := var n
+| (sort l)                    := sort l
+| (const nm ls)               := mk_explicit $ const nm ls
+| (mvar n n' e)               := mvar n n' (to_raw_pexpr e)
+| (local_const nm ppnm bi tp) := mk_explicit $ local_const nm ppnm bi (to_raw_pexpr tp)
+| (app f a)                   := app (to_raw_pexpr f) (to_raw_pexpr a)
+| (lam nm bi tp bd)           := lam nm bi (to_raw_pexpr tp) (to_raw_pexpr bd)
+| (pi nm bi tp bd)            := pi nm bi (to_raw_pexpr tp) (to_raw_pexpr bd)
+| (elet nm tp df bd)          := elet nm (to_raw_pexpr tp) (to_raw_pexpr df) (to_raw_pexpr bd)
+| (macro md l)                := macro md (l.map to_raw_pexpr)
+
+end expr open expr
+namespace pexpr
+meta def to_raw_expr : pexpr → expr
+| (var n)                     := var n
+| (sort l)                    := sort l
+| (const nm ls)               := const nm ls
+| (mvar n n' e)               := mvar n n' (to_raw_expr e)
+| (local_const nm ppnm bi tp) := local_const nm ppnm bi (to_raw_expr tp)
+| (app f a)                   := app (to_raw_expr f) (to_raw_expr a)
+| (lam nm bi tp bd)           := lam nm bi (to_raw_expr tp) (to_raw_expr bd)
+| (pi nm bi tp bd)            := pi nm bi (to_raw_expr tp) (to_raw_expr bd)
+| (elet nm tp df bd)          := elet nm (to_raw_expr tp) (to_raw_expr df) (to_raw_expr bd)
+| (macro md l)                := macro md (l.map to_raw_expr)
+
+end pexpr
 
 hott_theory
 
 namespace tactic
-open expr
+open interaction_monad interaction_monad.result sum
 
-open interaction_monad interaction_monad.result
+/-- Executes t, on failure the tactic try_core_msg succeeds with the error message -/
+meta def try_core_msg {α : Type _} (t : tactic α) : tactic (α ⊕ option (unit → format)) :=
+λ s, result.cases_on (t s)
+ (λ a, success $ inl a)
+ (λ e ref s', success (inr e) s)
+
+/-- Returns a if t returns (inl a), otherwise fails with message returned by t -/
+meta def extract {α : Type _} (t : tactic $ α ⊕ option (unit → format)) : tactic α :=
+do u ← t, 
+match u with
+| inl a        := return a
+| inr (some m) := fail $ m ()
+| inr none     := failed
+end
+
 
 /-- executes t₂ when tactic t₁ fails. After t₂ is executed, do_on_failure fails with the error message given by t₂ -/
 meta def do_on_failure {α : Type _} (t₁ : tactic α) (t₂ : format → tactic format) : tactic α :=
-λ s, match t₁ s with
-| (exception (some f) pos s') := (t₂ (f ()) >>= λx, exception (some $ λ_, x) pos) s'
-| (exception none pos s') := exception none pos s'
-| (interaction_monad.result.success a s') := interaction_monad.result.success a s'
+do r ← try_core_msg t₁,
+match r with
+| (inl a)        := return a
+| (inr none)     := do u ← t₂ "", fail u
+| (inr (some m)) := do u ← t₂ (m ()), fail u
+end
+
+/-- qlmost the same as t₁ <|> t₂. If t₂ returns value none, the tactic fails with error message from t₁ -/
+meta def orelse_plus {α : Type _} (t₁ : tactic α) (t₂ : tactic $ option α) : tactic α :=
+do r ← try_core_msg t₁,
+match r with
+| (inl a) := return a
+| (inr e) := do u ← t₂, some a ← return u | (do some u ← return e, fail $ u ()), return a
 end
 
 /-- change the error message on failure of t₁ -/
@@ -76,9 +116,21 @@ do e ← i_to_expr p,
    interactive.intro x,
    interactive.intro h
 
+/-- Binds local constant l in expression e. Infers the type of l for the binder type. 
+    Note: Does not instantiate metavariables, which might cause an incomplete abstraction. -/
+meta def bind_lambda (l e : expr) : tactic expr :=
+do t ← infer_type l,
+local_const un ppn bi _ ← return l | fail $ to_fmt l ++ " is not a local constant.",
+return $ lam (ppn.append_postfix "'") bi t (abstract_local e un)
+
+/- Binds local constants in expression e. Instantiates metavariables of e. -/
+meta def bind_lambdas : list expr → expr → tactic expr
+| []      e := instantiate_mvars e
+| (l::ls) e := do e' ← bind_lambdas ls e, bind_lambda l e'
+
 namespace interactive
 
-open lean lean.parser interactive
+open lean lean.parser interactive interactive.types
 local postfix `?`:9001 := optional
 
 meta def fconstructor : tactic unit :=
@@ -104,5 +156,42 @@ propagate_tags $ let (p, x) := p in tactic.hgeneralize h p x
 meta def trace_failure : itactic → tactic unit :=
 tactic.trace_failure
 
+meta def iapply (q : parse texpr) : tactic unit :=
+i_to_expr_for_apply q >>= (λe, tactic.apply e {instances := ff}) >> all_goals (try apply_instance)
+
 end interactive
 end tactic
+
+namespace list
+open tactic sum option
+meta def mmap_filter {α : Type u} {β : Type v} (f : α → tactic (option β)) : list α → tactic (list β)
+| []       := return []
+| (x :: xs) := do oy ← f x, ys ← mmap_filter xs, some y ← return oy | return ys, return $ y :: ys
+
+#print mfirst
+/-- Applies f to all elements of the list, until one of them returns (inl _). If f only returns (inr _) or fails this raises an error message which concatenates the returned messages. Discards messages of errors. Assumes that f always succeeds. -/
+meta def mfirst_msg_core {α : Type w} {β : Type} (f : α → tactic (β ⊕ option (unit → format))) : 
+  list α → list (unit → format) → tactic β
+| []      m := fail $ m.foldl (λm t, t () ++ "\n" ++ m) ""
+| (a::as) m := (do x ← f a, 
+  match x with 
+  | inl b := return b
+  | inr f := do x ← return f | mfirst_msg_core as m, mfirst_msg_core as m
+  end) <|> mfirst_msg_core as m
+
+meta def mfirst_msg {α : Type w} {β : Type} (f : α → tactic (β ⊕ option (unit → format))) (l : list α) : tactic β :=
+mfirst_msg_core f l []
+
+end list
+namespace option
+
+/-- The mmap for options. -/
+def mmap {m : Type u → Type v} [monad m] {α : Type w} {β : Type u} (f : α → m β) : option α → m (option β)
+| none     := return none
+| (some x) := do y ← f x, return $ some y
+
+def iget {α : Type u} [inhabited α] : option α → α
+| none     := default α
+| (some x) := x
+
+end option
