src/hott/init/path.lean
@@ -34,11 +34,11 @@ namespace eq
   /- Concatenation and inverse -/
   @[trans, hott]
   def concat (p : x = y) (q : y = z) : x = z :=
-  by induction q; exact p
+  by hinduction q; exact p
 
   @[symm, hott]
   def inverse (p : x = y) : y = x :=
-  by induction p; reflexivity
+  by hinduction p; reflexivity
 
   infix   ⬝  := concat
   postfix ⁻¹ := inverse
@@ -53,67 +53,67 @@ namespace eq
 
   -- The identity path is a left unit.
   @[hott, hsimp] def idp_con (p : x = y) : idp ⬝ p = p :=
-  by induction p; reflexivity
+  by hinduction p; reflexivity
 
   @[hott, hsimp] def idp_inv : (@idp _ x)⁻¹ = idp := idp
 
   -- Concatenation is associative.
   @[hott] def con.assoc (p : x = y) (q : y = z) (r : z = t) :
     (p ⬝ q) ⬝ r = p ⬝ (q ⬝ r) :=
-  by induction r; reflexivity
+  by hinduction r; reflexivity
 
-@[hott] def con.assoc' (p : x = y) (q : y = z) (r : z = t) :
+  @[hott] def con.assoc' (p : x = y) (q : y = z) (r : z = t) :
     p ⬝ (q ⬝ r) = (p ⬝ q) ⬝ r :=
   (con.assoc p q r)⁻¹
 
   @[hott] def con.assoc5 {a₁ a₂ a₃ a₄ a₅ a₆ : A}
     (p₁ : a₁ = a₂) (p₂ : a₂ = a₃) (p₃ : a₃ = a₄) (p₄ : a₄ = a₅) (p₅ : a₅ = a₆) :
     p₁ ⬝ (p₂ ⬝ p₃ ⬝ p₄) ⬝ p₅ = (p₁ ⬝ p₂) ⬝ p₃ ⬝ (p₄ ⬝ p₅) :=
-  by induction p₅; induction p₄; induction p₃; reflexivity
+  by hinduction p₅; hinduction p₄; hinduction p₃; reflexivity
 
   -- The left inverse law.
   @[hott, hsimp] def con.right_inv (p : x = y) : p ⬝ p⁻¹ = idp :=
-  by induction p; reflexivity
+  by hinduction p; reflexivity
 
   -- The right inverse law.
   @[hott, hsimp] def con.left_inv (p : x = y) : p⁻¹ ⬝ p = idp :=
-  by induction p; reflexivity
+  by hinduction p; reflexivity
 
   /- Several auxiliary theorems about canceling inverses across associativity. These are somewhat
      redundant, following from earlier theorems. -/
 
   @[hott, hsimp] def inv_con_cancel_left (p : x = y) (q : y = z) : p⁻¹ ⬝ (p ⬝ q) = q :=
-  by induction q; induction p; reflexivity
+  by hinduction q; hinduction p; reflexivity
 
   @[hott, hsimp] def con_inv_cancel_left (p : x = y) (q : x = z) : p ⬝ (p⁻¹ ⬝ q) = q :=
-  by induction q; induction p; reflexivity
+  by hinduction q; hinduction p; reflexivity
 
   @[hott, hsimp] def con_inv_cancel_right (p : x = y) (q : y = z) : (p ⬝ q) ⬝ q⁻¹ = p :=
-  by induction q; reflexivity
+  by hinduction q; reflexivity
 
   @[hott, hsimp] def inv_con_cancel_right (p : x = z) (q : y = z) : (p ⬝ q⁻¹) ⬝ q = p :=
-  by induction q; reflexivity
+  by hinduction q; reflexivity
 
   -- Inverse distributes over concatenation
   @[hott]
   def con_inv (p : x = y) (q : y = z) : (p ⬝ q)⁻¹ = q⁻¹ ⬝ p⁻¹ :=
-  by induction q; induction p; reflexivity
+  by hinduction q; hinduction p; reflexivity
 
   @[hott]
   def inv_con_inv_left (p : y = x) (q : y = z) : (p⁻¹ ⬝ q)⁻¹ = q⁻¹ ⬝ p :=
-  by induction q; induction p; reflexivity
+  by hinduction q; hinduction p; reflexivity
 
   @[hott]
   def inv_con_inv_right (p : x = y) (q : z = y) : (p ⬝ q⁻¹)⁻¹ = q ⬝ p⁻¹ :=
-  by induction q; induction p; reflexivity
+  by hinduction q; hinduction p; reflexivity
 
   @[hott]
   def inv_con_inv_inv (p : y = x) (q : z = y) : (p⁻¹ ⬝ q⁻¹)⁻¹ = q ⬝ p :=
-  by induction q; induction p; reflexivity
+  by hinduction q; hinduction p; reflexivity
 
   -- Inverse is an involution.
   @[hott, hsimp] def inv_inv  (p : x = y) : p⁻¹⁻¹ = p :=
-  by induction p; reflexivity
+  by hinduction p; reflexivity
 
   -- auxiliary def used by 'cases' tactic
   @[hott]
@@ -123,7 +123,7 @@ namespace eq
 
   @[hott] def eq.rec_symm {A : Type u} {a₀ : A} {P : Π⦃a₁⦄, a₁ = a₀ → Type v}
     (H : P idp) ⦃a₁ : A⦄ (p : a₁ = a₀) : P p :=
-  by induction p; exact H
+  by hinduction p; exact H
 
   /- Theorems for moving things around in equations -/
 
@@ -133,100 +133,100 @@ namespace eq
   def con_eq_of_eq_inv_con {p : x = z} {q : y = z} {r : y = x} :
     p = r⁻¹ ⬝ q → r ⬝ p = q :=
   begin
-    induction r, intro h, exact !idp_con ⬝ h ⬝ !idp_con
+    hinduction r, intro h, exact !idp_con ⬝ h ⬝ !idp_con
   end
 
   @[hott]
   def con_eq_of_eq_con_inv  {p : x = z} {q : y = z} {r : y = x} :
     r = q ⬝ p⁻¹ → r ⬝ p = q :=
-  by induction p; exact id
+  by hinduction p; exact id
 
   @[hott]
   def inv_con_eq_of_eq_con {p : x = z} {q : y = z} {r : x = y} :
     p = r ⬝ q → r⁻¹ ⬝ p = q :=
-  by induction r; intro h; exact !idp_con ⬝ h ⬝ !idp_con
+  by hinduction r; intro h; exact !idp_con ⬝ h ⬝ !idp_con
 
   @[hott]
   def con_inv_eq_of_eq_con  {p : z = x} {q : y = z} {r : y = x} :
     r = q ⬝ p → r ⬝ p⁻¹ = q :=
-  by induction p; exact id
+  by hinduction p; exact id
 
   @[hott] def eq_con_of_inv_con_eq {p : x = z} {q : y = z} {r : y = x} :
     r⁻¹ ⬝ q = p → q = r ⬝ p :=
-  by induction r; intro h; exact !idp_con⁻¹ ⬝ h ⬝ !idp_con⁻¹
+  by hinduction r; intro h; exact !idp_con⁻¹ ⬝ h ⬝ !idp_con⁻¹
 
   @[hott] def eq_con_of_con_inv_eq  {p : x = z} {q : y = z} {r : y = x} :
     q ⬝ p⁻¹ = r → q = r ⬝ p :=
-  by induction p; exact id
+  by hinduction p; exact id
 
   @[hott] def eq_inv_con_of_con_eq {p : x = z} {q : y = z} {r : x = y} :
     r ⬝ q = p → q = r⁻¹ ⬝ p :=
-  by induction r; intro h; exact !idp_con⁻¹ ⬝ h ⬝ !idp_con⁻¹
+  by hinduction r; intro h; exact !idp_con⁻¹ ⬝ h ⬝ !idp_con⁻¹
 
   @[hott] def eq_con_inv_of_con_eq  {p : z = x} {q : y = z} {r : y = x} :
     q ⬝ p = r → q = r ⬝ p⁻¹ :=
-  by induction p; exact id
+  by hinduction p; exact id
 
   @[hott] def eq_of_con_inv_eq_idp  {p q : x = y} : p ⬝ q⁻¹ = idp → p = q :=
-  by induction q; exact id
+  by hinduction q; exact id
 
   @[hott] def eq_of_inv_con_eq_idp {p q : x = y} : q⁻¹ ⬝ p = idp → p = q :=
-  by induction q; intro h; exact !idp_con⁻¹ ⬝ h
+  by hinduction q; intro h; exact !idp_con⁻¹ ⬝ h
 
   @[hott] def eq_inv_of_con_eq_idp'  {p : x = y} {q : y = x} : p ⬝ q = idp → p = q⁻¹ :=
-  by induction q; exact id
+  by hinduction q; exact id
 
   @[hott] def eq_inv_of_con_eq_idp {p : x = y} {q : y = x} : q ⬝ p = idp → p = q⁻¹ :=
-  by induction q; intro h; exact !idp_con⁻¹ ⬝ h
+  by hinduction q; intro h; exact !idp_con⁻¹ ⬝ h
 
   @[hott] def eq_of_idp_eq_inv_con {p q : x = y} : idp = p⁻¹ ⬝ q → p = q :=
-  by induction p; intro h; exact h ⬝ !idp_con
+  by hinduction p; intro h; exact h ⬝ !idp_con
 
   @[hott] def eq_of_idp_eq_con_inv  {p q : x = y} : idp = q ⬝ p⁻¹ → p = q :=
-  by induction p; exact id
+  by hinduction p; exact id
 
   @[hott] def inv_eq_of_idp_eq_con  {p : x = y} {q : y = x} : idp = q ⬝ p → p⁻¹ = q :=
-  by induction p; exact id
+  by hinduction p; exact id
 
   @[hott] def inv_eq_of_idp_eq_con' {p : x = y} {q : y = x} : idp = p ⬝ q → p⁻¹ = q :=
-  by induction p; intro h; exact h ⬝ !idp_con
+  by hinduction p; intro h; exact h ⬝ !idp_con
 
   @[hott] def con_inv_eq_idp  {p q : x = y} (r : p = q) : p ⬝ q⁻¹ = idp :=
-  by induction r; apply con.right_inv
+  by hinduction r; apply con.right_inv
 
   @[hott] def inv_con_eq_idp  {p q : x = y} (r : p = q) : q⁻¹ ⬝ p = idp :=
-  by induction r; apply con.left_inv
+  by hinduction r; apply con.left_inv
 
   @[hott] def con_eq_idp {p : x = y} {q : y = x} (r : p = q⁻¹) : p ⬝ q = idp :=
-  by induction q; exact r
+  by hinduction q; exact r
 
   @[hott] def idp_eq_inv_con {p q : x = y} (r : p = q) : idp = p⁻¹ ⬝ q :=
-  by induction r; exact (con.left_inv _)⁻¹
+  by hinduction r; exact (con.left_inv _)⁻¹
 
   @[hott] def idp_eq_con_inv {p q : x = y} (r : p = q) : idp = q ⬝ p⁻¹ :=
-  by induction r; exact (con.right_inv _)⁻¹
+  by hinduction r; exact (con.right_inv _)⁻¹
 
   @[hott] def idp_eq_con {p : x = y} {q : y = x} (r : p⁻¹ = q) : idp = q ⬝ p :=
-  by induction p; exact r
+  by hinduction p; exact r
 
   @[hott] def eq_idp_of_con_right {p : x = x} {q : x = y} (r : p ⬝ q = q) : p = idp :=
-  by induction q; exact r
+  by hinduction q; exact r
 
   @[hott] def eq_idp_of_con_left {p : x = x} {q : y = x} (r : q ⬝ p = q) : p = idp :=
-  by induction q; exact (idp_con p)⁻¹ ⬝ r
+  by hinduction q; exact (idp_con p)⁻¹ ⬝ r
 
   @[hott] def idp_eq_of_con_right {p : x = x} {q : x = y} (r : q = p ⬝ q) : idp = p :=
-  by induction q; exact r
+  by hinduction q; exact r
 
   @[hott] def idp_eq_of_con_left {p : x = x} {q : y = x} (r : q = q ⬝ p) : idp = p :=
-  by induction q; exact r ⬝ idp_con p
+  by hinduction q; exact r ⬝ idp_con p
 
   /- Transport -/
 
   @[subst, hott, elab_simple]
-  def transport (P : A → Sort v) {x y : A} (p : x = y)
+  def transport (P : A → Type v) {x y : A} (p : x = y)
     (u : P x) : P y :=
-  by induction p; exact u
+  by hinduction p; exact u
 
   -- This idiom makes the operation right associative.
   hott_theory_cmd "local infixr ` ▸ ` := hott.eq.transport _"
@@ -245,7 +245,7 @@ namespace eq
   p⁻¹ ▸ u
 
   @[hott, elab_simple] def ap {{A : Type u}} {{B : Type v}} (f : A → B) {x y:A} (p : x = y) : f x = f y :=
-  by induction p; reflexivity
+  by hinduction p; reflexivity
 
   @[hott, hsimp] def eq_rec_ap {A B} (f : A → B) {x y : A} (p : x = y) :
     (eq.rec idp p : f x = f y) = ap f p := idp
@@ -306,52 +306,52 @@ namespace eq
   transport (λ g, f ~ g) H1 (homotopy.refl f)
 
   @[hott, elab_simple] def apd10  {f g : Πx, P x} (H : f = g) : f ~ g :=
-  λx, by induction H; reflexivity
+  λx, by hinduction H; reflexivity
 
   --the next theorem is useful if you want to write "apply (apd10' a)"
   @[hott] def apd10'  {f g : Πx, P x} (a : A) (H : f = g) : f a = g a :=
-  by induction H; reflexivity
+  by hinduction H; reflexivity
 
   --apd10 is also ap evaluation
   @[hott] def apd10_eq_ap_eval {f g : Πx, P x} (H : f = g) (a : A)
     : apd10 H a = ap (λs : Πx, P x, s a) H :=
-  by induction H; reflexivity
+  by hinduction H; reflexivity
 
   @[reducible,hott]
   def ap10 {f g : A → B} (H : f = g) : f ~ g := apd10 H
 
   @[hott, congr] def ap11 {f g : A → B} (H : f = g) {x y : A} (p : x = y) : f x = g y :=
-  by induction H; exact ap f p
+  by hinduction H; exact ap f p
 
   -- [apd] is defined in init.pathover using pathover instead of an equality with transport.
   @[hott] def apdt  (f : Πa, P a) {x y : A} (p : x = y) : p ▸ f x = f y :=
-  by induction p; reflexivity
+  by hinduction p; reflexivity
 
   @[hott, elab_simple] def ap011  (f : A → B → C) (Ha : a = a') (Hb : b = b') : f a b = f a' b' :=
-  by induction Ha; exact ap (f a) Hb
+  by hinduction Ha; exact ap (f a) Hb
 
   /- More theorems for moving things around in equations -/
 
   @[hott] def tr_eq_of_eq_inv_tr {P : A → Type v} {x y : A} {p : x = y} {u : P x} {v : P y} :
     u = p⁻¹ ▸ v → p ▸ u = v :=
-  by induction p; exact id
+  by hinduction p; exact id
 
   @[hott] def inv_tr_eq_of_eq_tr {P : A → Type v} {x y : A} {p : y = x} {u : P x} {v : P y} :
     u = p ▸ v → p⁻¹ ▸ u = v :=
-  by induction p; exact id
+  by hinduction p; exact id
 
   @[hott] def eq_inv_tr_of_tr_eq {P : A → Type v} {x y : A} {p : x = y} {u : P x} {v : P y} :
     p ▸ u = v → u = p⁻¹ ▸ v :=
-  by induction p; exact id
+  by hinduction p; exact id
 
   @[hott] def eq_tr_of_inv_tr_eq {P : A → Type v} {x y : A} {p : y = x} {u : P x} {v : P y} :
     p⁻¹ ▸ u = v → u = p ▸ v :=
-  by induction p; exact id
+  by hinduction p; exact id
 
   /- Transporting along the diagonal of a type family -/
   @[hott] def tr_diag_eq_tr_tr {A : Type u} (P : A → A → Type v) {x y : A} (p : x = y) (a : P x x) :
     transport (λ x, P x x) p a = transport (λ z, P y z) p (@transport _ (λ z, P z x) _ _ p a) :=
-  by induction p; reflexivity
+  by hinduction p; reflexivity
 
   /- Functoriality of functions -/
 
@@ -364,112 +364,112 @@ namespace eq
   -- Functions commute with concatenation.
   @[hott] def ap_con  (f : A → B) {x y z : A} (p : x = y) (q : y = z) :
     ap f (p ⬝ q) = ap f p ⬝ ap f q :=
-  by induction q; reflexivity
+  by hinduction q; reflexivity
 
   @[hott] def con_ap_con_eq_con_ap_con_ap (f : A → B) {w x y z : A} (r : f w = f x)
     (p : x = y) (q : y = z) : r ⬝ ap f (p ⬝ q) = (r ⬝ ap f p) ⬝ ap f q :=
-  by induction q; induction p; reflexivity
+  by hinduction q; hinduction p; reflexivity
 
   @[hott] def ap_con_con_eq_ap_con_ap_con (f : A → B) {w x y z : A} (p : x = y) (q : y = z)
     (r : f z = f w) : ap f (p ⬝ q) ⬝ r = ap f p ⬝ (ap f q ⬝ r) :=
-  begin induction q; induction p, exact (idp_con _)⁻¹ end
+  begin hinduction q; hinduction p, exact (idp_con _)⁻¹ end
 
   -- Functions commute with path inverses.
   @[hott] def ap_inv'  (f : A → B) {x y : A} (p : x = y) : (ap f p)⁻¹ = ap f p⁻¹ :=
-  by induction p; reflexivity
+  by hinduction p; reflexivity
 
   @[hott] def ap_inv  (f : A → B) {x y : A} (p : x = y) : ap f p⁻¹ = (ap f p)⁻¹ :=
-  by induction p; reflexivity
+  by hinduction p; reflexivity
 
   -- [ap] itself is functorial in the first argument.
 
   @[hott, hsimp] def ap_id  (p : x = y) : ap id p = p :=
-  by induction p; reflexivity
+  by hinduction p; reflexivity
 
   @[hott,elab_simple] def ap_compose  (g : B → C) (f : A → B) {x y : A} (p : x = y) :
     ap (g ∘ f) p = (ap g (ap f p) : g (f x) = g (f y)) :=
-  by induction p; reflexivity
+  by hinduction p; reflexivity
 
   -- Sometimes we don't have the actual function [compose].
   @[hott] def ap_compose'  (g : B → C) (f : A → B) {x y : A} (p : x = y) :
     ap g (ap f p) = ap (λa, g (f a)) p :=
-  by induction p; reflexivity
+  by hinduction p; reflexivity
 
   -- The action of constant maps.
   @[hott] def ap_constant  (p : x = y) (z : B) : ap (λu, z) p = idp :=
-  by induction p; reflexivity
+  by hinduction p; reflexivity
 
   -- Naturality of [ap].
   -- see also natural_square in cubical.square
   @[hott] def ap_con_eq_con_ap {f g : A → B} (p : f ~ g) {x y : A} (q : x = y) :
     ap f q ⬝ p y = p x ⬝ ap g q :=
-  by induction q; apply idp_con
+  by hinduction q; apply idp_con
 
   -- Naturality of [ap] at identity.
   @[hott] def ap_con_eq_con {f : A → A} (p : Πx, f x = x) {x y : A} (q : x = y) :
     ap f q ⬝ p y = p x ⬝ q :=
-  by induction q; apply idp_con
+  by hinduction q; apply idp_con
 
   @[hott] def con_ap_eq_con {f : A → A} (p : Πx, x = f x) {x y : A} (q : x = y) :
     p x ⬝ ap f q =  q ⬝ p y :=
-  by induction q; exact !idp_con⁻¹
+  by hinduction q; exact !idp_con⁻¹
 
   -- Naturality of [ap] with constant function
   @[hott] def ap_con_eq {f : A → B} {b : B} (p : Πx, f x = b) {x y : A} (q : x = y) :
     ap f q ⬝ p y = p x :=
-  by induction q; apply idp_con
+  by hinduction q; apply idp_con
 
   -- Naturality with other paths hanging around.
 
   @[hott] def con_ap_con_con_eq_con_con_ap_con {f g : A → B} (p : f ~ g) {x y : A} (q : x = y)
       {w z : B} (r : w = f x) (s : g y = z) :
     (r ⬝ ap f q) ⬝ (p y ⬝ s) = (r ⬝ p x) ⬝ (ap g q ⬝ s) :=
-  by induction s; induction q; reflexivity
+  by hinduction s; hinduction q; reflexivity
 
   @[hott] def con_ap_con_eq_con_con_ap {f g : A → B} (p : f ~ g) {x y : A} (q : x = y)
       {w : B} (r : w = f x) :
     (r ⬝ ap f q) ⬝ p y = (r ⬝ p x) ⬝ ap g q :=
-  by induction q; reflexivity
+  by hinduction q; reflexivity
 
   -- TODO: try this using the simplifier, and compare proofs
   @[hott] def ap_con_con_eq_con_ap_con {f g : A → B} (p : f ~ g) {x y : A} (q : x = y)
       {z : B} (s : g y = z) :
     ap f q ⬝ (p y ⬝ s) = p x ⬝ (ap g q ⬝ s) :=
   begin
-    induction s,
-    induction q,
+    hinduction s,
+    hinduction q,
     apply idp_con
   end
 
   @[hott] def con_ap_con_con_eq_con_con_con {f : A → A} (p : f ~ id) {x y : A} (q : x = y)
       {w z : A} (r : w = f x) (s : y = z) :
     (r ⬝ ap f q) ⬝ (p y ⬝ s) = (r ⬝ p x) ⬝ (q ⬝ s) :=
-  by induction s; induction q; reflexivity
+  by hinduction s; hinduction q; reflexivity
 
   @[hott] def con_con_ap_con_eq_con_con_con {g : A → A} (p : @id A ~ g) {x y : A} (q : x = y)
       {w z : A} (r : w = x) (s : g y = z) :
     (r ⬝ p x) ⬝ (ap g q ⬝ s) = (r ⬝ q) ⬝ (p y ⬝ s) :=
-  by induction s; induction q; reflexivity
+  by hinduction s; hinduction q; reflexivity
 
   @[hott] def con_ap_con_eq_con_con {f : A → A} (p : f ~ id) {x y : A} (q : x = y)
       {w : A} (r : w = f x) :
     (r ⬝ ap f q) ⬝ p y = (r ⬝ p x) ⬝ q :=
-  by induction q; reflexivity
+  by hinduction q; reflexivity
 
   @[hott] def ap_con_con_eq_con_con {f : A → A} (p : f ~ id) {x y : A} (q : x = y)
       {z : A} (s : y = z) :
     ap f q ⬝ (p y ⬝ s) = p x ⬝ (q ⬝ s) :=
-  by induction s; induction q; apply idp_con
+  by hinduction s; hinduction q; apply idp_con
 
   @[hott] def con_con_ap_eq_con_con {g : A → A} (p : @id A ~ g) {x y : A} (q : x = y)
       {w : A} (r : w = x) :
     (r ⬝ p x) ⬝ ap g q = (r ⬝ q) ⬝ p y :=
-  begin induction q, exact idp end
+  begin hinduction q, exact idp end
 
   @[hott] def con_ap_con_eq_con_con' {g : A → A} (p : @id A ~ g) {x y : A} (q : x = y)
       {z : A} (s : g y = z) :
     p x ⬝ (ap g q ⬝ s) = q ⬝ (p y ⬝ s) :=
-  by induction s; induction q; exact !idp_con⁻¹
+  by hinduction s; hinduction q; exact !idp_con⁻¹
 
   /- Action of [apd10] and [ap10] on paths -/
 
@@ -479,11 +479,11 @@ namespace eq
 
   @[hott] def apd10_con {f f' f'' : Πx, P x} (h : f = f') (h' : f' = f'') (x : A) :
     apd10 (h ⬝ h') x = apd10 h x ⬝ apd10 h' x :=
-  by induction h; induction h'; reflexivity
+  by hinduction h; hinduction h'; reflexivity
 
   @[hott] def apd10_inv {f g : Πx : A, P x} (h : f = g) (x : A) :
     apd10 h⁻¹ x = (apd10 h x)⁻¹ :=
-  by induction h; reflexivity
+  by hinduction h; reflexivity
 
   @[hott, hsimp] def ap10_idp {f : A → B} (x : A) : ap10 (refl f) x = idp := idp
 
@@ -496,13 +496,13 @@ namespace eq
   -- [ap10] also behaves nicely on paths produced by [ap]
   @[hott] def ap_ap10 (f g : A → B) (h : B → C) (p : f = g) (a : A) :
     ap h (ap10 p a) = ap10 (ap (λ f' : A → B, h ∘ f') p) a:=
-  by induction p; reflexivity
+  by hinduction p; reflexivity
 
   /- some lemma's about ap011 -/
 
   @[hott] def ap_eq_ap011_left (f : A → B → C) (Ha : a = a') (b : B) :
     ap (λa, f a b) Ha = ap011 f Ha idp :=
-  by induction Ha; reflexivity
+  by hinduction Ha; reflexivity
 
   @[hott] def ap_eq_ap011_right (f : A → B → C) (a : A) (Hb : b = b') :
     ap (f a) Hb = ap011 f idp Hb :=
@@ -511,7 +511,7 @@ namespace eq
   @[hott] def ap_ap011 {A B C D : Type _} (g : C → D) (f : A → B → C) {a a' : A} {b b' : B}
     (p : a = a') (q : b = b') : ap g (ap011 f p q) = ap011 (λa b, g (f a b)) p q :=
   begin
-    induction p, exact (ap_compose g (f a) q)⁻¹
+    hinduction p, exact (ap_compose g (f a) q)⁻¹
   end
 
 
@@ -521,7 +521,7 @@ namespace eq
 
   @[hott] def con_tr  {P : A → Type w} {x y z : A} (p : x = y) (q : y = z) (u : P x) :
     p ⬝ q ▸ u = q ▸ p ▸ u :=
-  by induction q; reflexivity
+  by hinduction q; reflexivity
 
   @[hott, hsimp] def tr_inv_tr {P : A → Type v} {x y : A} (p : x = y) (z : P y) :
     p ▸ p⁻¹ ▸ z = z :=
@@ -533,19 +533,19 @@ namespace eq
 
   @[hott] def cast_cast_inv {A : Type u} {P : A → Type u} {x y : A} (p : x = y) (z : P y) :
     cast (ap P p) (cast (ap P p⁻¹) z) = z :=
-  by induction p; reflexivity
+  by hinduction p; reflexivity
 
   @[hott] def cast_inv_cast {A : Type u} {P : A → Type u} {x y : A} (p : x = y) (z : P x) :
     cast (ap P p⁻¹) (cast (ap P p) z) = z :=
-  by induction p; reflexivity
+  by hinduction p; reflexivity
 
   @[hott] def fn_tr_eq_tr_fn {P Q : A → Type _} {x y : A} (p : x = y) (f : Πx, P x → Q x) (z : P x) :
     f y (p ▸ z) = p ▸ f x z :=
-  by induction p; reflexivity
+  by hinduction p; reflexivity
 
   @[hott] def fn_cast_eq_cast_fn {A : Type _} {P Q : A → Type _} {x y : A} (p : x = y)
     (f : Πx, P x → Q x) (z : P x) : f y (cast (ap P p) z) = cast (ap Q p) (f x z) :=
-  by induction p; reflexivity
+  by hinduction p; reflexivity
 
   @[hott] def con_con_tr {P : A → Type u}
       {x y z w : A} (p : x = y) (q : y = z) (r : z = w) (u : P x) :
@@ -553,12 +553,12 @@ namespace eq
         ap (transport P r) (con_tr p q u)
       = con_tr p (q ⬝ r) u ⬝ con_tr q r (p ▸ u)
       :> ((p ⬝ (q ⬝ r)) ▸ u = r ▸ q ▸ p ▸ u) :=
-  by induction r; induction q; induction p; reflexivity
+  by hinduction r; hinduction q; hinduction p; reflexivity
 
   --  Here is another coherence lemma for transport.
   @[hott] def tr_inv_tr_lemma {P : A → Type v} {x y : A} (p : x = y) (z : P x) :
     tr_inv_tr p (transport P p z) = ap (transport P p) (inv_tr_tr p z) :=
-  by induction p; reflexivity
+  by hinduction p; reflexivity
 
   /- some properties for apdt -/
 
@@ -566,17 +566,17 @@ namespace eq
 
   @[hott] def apdt_con (f : Πx, P x) {x y z : A} (p : x = y) (q : y = z)
     : apdt f (p ⬝ q) = con_tr p q (f x) ⬝ ap (transport P q) (apdt f p) ⬝ apdt f q :=
-  by induction p; induction q; apply idp
+  by hinduction p; hinduction q; apply idp
 
   @[hott] def apdt_inv (f : Πx, P x) {x y : A} (p : x = y)
     : apdt f p⁻¹ = (eq_inv_tr_of_tr_eq (apdt f p))⁻¹ :=
-  by induction p; apply idp
+  by hinduction p; apply idp
 
   -- Dependent transport in a doubly dependent type.
   -- This is a special case of transporto in init.pathover
   @[hott] def transportD  {P : A → Type _} (Q : Πa, P a → Type _)
       {a a' : A} (p : a = a') (b : P a) (z : Q a b) : Q a' (p ▸ b) :=
-  by induction p; exact z
+  by hinduction p; exact z
 
   -- In Coq the variables P, Q and b are explicit, but in Lean we can probably have them implicit
   -- using the following notation
@@ -598,27 +598,27 @@ namespace eq
   -- An alternative definition.
   @[hott] def tr2_eq_ap10 (Q : A → Type w) {x y : A} {p q : x = y} (r : p = q) (z : Q x) :
     transport2 Q r z = ap10 (ap (transport Q) r) z :=
-  by induction r; reflexivity
+  by hinduction r; reflexivity
 
   @[hott] def tr2_con {P : A → Type w} {x y : A} {p1 p2 p3 : x = y}
       (r1 : p1 = p2) (r2 : p2 = p3) (z : P x) :
     transport2 P (r1 ⬝ r2) z = transport2 P r1 z ⬝ transport2 P r2 z :=
-  by induction r1; induction r2; reflexivity
+  by hinduction r1; hinduction r2; reflexivity
 
   @[hott] def tr2_inv (Q : A → Type w) {x y : A} {p q : x = y} (r : p = q) (z : Q x) :
     transport2 Q r⁻¹ z = (transport2 Q r z)⁻¹ :=
-  by induction r; reflexivity
+  by hinduction r; reflexivity
 
   @[hott] def transportD2  {B C : A → Type _} (D : Π(a:A), B a → C a → Type _)
     {x1 x2 : A} (p : x1 = x2) (y : B x1) (z : C x1) (w : D x1 y z) : D x2 (p ▸ y) (p ▸ z) :=
-  by induction p; exact w
+  by hinduction p; exact w
 
   notation p ` ▸D2 `:65 x:64 := transportD2 _ p _ _ x
 
   @[hott] def ap_tr_con_tr2 (P : A → Type _) {x y : A} {p q : x = y} {z w : P x} (r : p = q)
       (s : z = w) :
     ap (transport P p) s  ⬝  transport2 P r w = transport2 P r z  ⬝  ap (transport P q) s :=
-  by induction r; exact !idp_con⁻¹
+  by hinduction r; exact !idp_con⁻¹
 
   /- Transporting in particular fibrations -/
 
@@ -633,16 +633,16 @@ namespace eq
 
   -- Transporting in a constant fibration.
   @[hott] def tr_constant (p : x = y) (z : B) : transport (λx, B) p z = z :=
-  by induction p; reflexivity
+  by hinduction p; reflexivity
 
   @[hott] def tr2_constant {p q : x = y} (r : p = q) (z : B) :
     tr_constant p z = transport2 (λu, B) r z ⬝ tr_constant q z :=
-  by induction r; exact !idp_con⁻¹
+  by hinduction r; exact !idp_con⁻¹
 
   -- Transporting in a pulled back fibration.
   @[hott] def tr_compose (P : B → Type _) (f : A → B) (p : x = y) (z : P (f x)) :
     transport (P ∘ f) p z  = transport P (ap f p) z :=
-  by induction p; reflexivity
+  by hinduction p; reflexivity
 
   @[hott] def tr_ap (P : B → Type _) (f : A → B) (p : x = y) (z : P (f x)) :
     transport P (ap f p) z = transport (P ∘ f) p z :=
@@ -650,34 +650,34 @@ namespace eq
 
   @[hott] def ap_precompose (f : A → B) (g g' : B → C) (p : g = g') :
     ap (λh : B → C, h ∘ f) p = transport (λh : B → C, g ∘ f = h ∘ f) p idp :=
-  by induction p; reflexivity
+  by hinduction p; reflexivity
 
   @[hott] def apd10_ap_precompose (f : A → B) (g g' : B → C) (p : g = g') :
     apd10 (ap (λh : B → C, h ∘ f) p) = λa, apd10 p (f a) :=
-  by induction p; reflexivity
+  by hinduction p; reflexivity
 
   @[hott] def apd10_ap_precompose_dependent {C : B → Type _}
     (f : A → B) {g g' : Πb : B, C b} (p : g = g')
     : apd10 (ap (λ(h : (Πb : B, C b))(a : A), h (f a)) p) = λa, apd10 p (f a) :=
-  by induction p; reflexivity
+  by hinduction p; reflexivity
 
   @[hott] def apd10_ap_postcompose (f : B → C) (g g' : A → B) (p : g = g') :
     apd10 (ap (λh : A → B, f ∘ h) p) = λa, ap f (apd10 p a) :=
-  by induction p; reflexivity
+  by hinduction p; reflexivity
 
   -- A special case of [tr_compose] which seems to come up a lot.
   @[hott] def tr_eq_cast_ap {P : A → Type _} {x y} (p : x = y) (u : P x) : p ▸ u = cast (ap P p) u :=
   tr_compose id P p u
 
   @[hott] def tr_eq_cast_ap_fn {P : A → Type _} {x y} (p : x = y) : transport P p = cast (ap P p) :=
-  by induction p; reflexivity
+  by hinduction p; reflexivity
 
   /- The behavior of [ap] and [apdt] -/
 
   -- In a constant fibration, [apdt] reduces to [ap], modulo [transport_const].
   @[hott] def apdt_eq_tr_constant_con_ap (f : A → B) (p : x = y) :
     apdt f p = tr_constant p (f x) ⬝ ap f p :=
-  by induction p; reflexivity
+  by hinduction p; reflexivity
 
 
   /- The 2-dimensional groupoid structure -/
@@ -714,7 +714,7 @@ namespace eq
 
   @[hott, hsimp] def whisker_right_idp {p q : x = y} (h : p = q) :
     whisker_right idp h = h :=
-  by induction h; induction p; reflexivity
+  by hinduction h; hinduction p; reflexivity
 
   @[hott, hsimp] def whisker_right_idp_left  (p : x = y) (q : y = z) :
     whisker_right q idp = idp :> (p ⬝ q = p ⬝ q) :=
@@ -726,7 +726,7 @@ namespace eq
 
   @[hott, hsimp] def whisker_left_idp {p q : x = y} (h : p = q) :
     (idp_con p)⁻¹ ⬝ whisker_left idp h ⬝ idp_con q = h :=
-  by induction h; induction p; reflexivity
+  by hinduction h; hinduction p; reflexivity
 
   @[hott, hsimp] def whisker_left_idp2 {A : Type u} {a : A} (p : idp = idp :> a = a) :
     whisker_left idp p = p :=
@@ -745,26 +745,26 @@ namespace eq
 
   @[hott] def inv2_con2 {p p' : x = y} (h : p = p')
     : h⁻² ◾ h = con.left_inv p ⬝ (con.left_inv p')⁻¹ :=
-  by induction h; induction p; reflexivity
+  by hinduction h; hinduction p; reflexivity
 
   -- The interchange law for concatenation.
   @[hott] def con2_con_con2 {p p' p'' : x = y} {q q' q'' : y = z}
       (a : p = p') (b : p' = p'') (c : q = q') (d : q' = q'') :
     a ◾ c ⬝ b ◾ d = (a ⬝ b) ◾ (c ⬝ d) :=
-  by induction d; induction c; induction b;induction a; reflexivity
+  by hinduction d; hinduction c; hinduction b;induction a; reflexivity
 
   @[hott] def con2_eq_rl {A : Type _} {x y z : A} {p p' : x = y} {q q' : y = z}
     (a : p = p') (b : q = q') : a ◾ b = whisker_right q a ⬝ whisker_left p' b :=
-  by induction b; induction a; reflexivity
+  by hinduction b; hinduction a; reflexivity
 
   @[hott] def con2_eq_lf {A : Type _} {x y z : A} {p p' : x = y} {q q' : y = z}
     (a : p = p') (b : q = q') : a ◾ b = whisker_left p b ⬝ whisker_right q' a :=
-  by induction b; induction a; reflexivity
+  by hinduction b; hinduction a; reflexivity
 
   @[hott] def whisker_right_con_whisker_left {x y z : A} {p p' : x = y} {q q' : y = z}
     (a : p = p') (b : q = q') :
     (whisker_right q a) ⬝ (whisker_left p' b) = (whisker_left p b) ⬝ (whisker_right q' a) :=
-  by induction b; induction a; reflexivity
+  by hinduction b; hinduction a; reflexivity
 
   -- Structure corresponding to the coherence equations of a bicategory.
 
@@ -774,12 +774,12 @@ namespace eq
       ⬝ con.assoc' p (q ⬝ r) s
       ⬝ whisker_right s (con.assoc' p q r)
     = con.assoc' p q (r ⬝ s) ⬝ con.assoc' (p ⬝ q) r s :=
-  by induction s;induction r;induction q;induction p;reflexivity
+  by hinduction s;induction r;induction q;induction p;reflexivity
 
   -- The 3-cell witnessing the left unit triangle.
   @[hott] def triangulator (p : x = y) (q : y = z) :
     con.assoc' p idp q ⬝ whisker_right q (con_idp p) = whisker_left p (idp_con q) :=
-  by induction q; induction p; reflexivity
+  by hinduction q; hinduction p; reflexivity
 
   @[hott] def eckmann_hilton (p q : idp = idp :> a = a) : p ⬝ q = q ⬝ p :=
   begin
@@ -810,18 +810,18 @@ namespace eq
 
   @[hott] def ap02_con (f : A → B) {x y : A} {p p' p'' : x = y} (r : p = p') (r' : p' = p'') :
     ap02 f (r ⬝ r') = ap02 f r ⬝ ap02 f r' :=
-  by induction r; induction r'; reflexivity
+  by hinduction r; hinduction r'; reflexivity
 
   @[hott] def ap02_con2 (f : A → B) {x y z : A} {p p' : x = y} {q q' :y = z} (r : p = p')
     (s : q = q') :
       ap02 f (r ◾ s) = ap_con f p q
                         ⬝ (ap02 f r ◾ ap02 f s)
                         ⬝ (ap_con f p' q')⁻¹ :=
-  by induction r; induction s; induction q; induction p; reflexivity
+  by hinduction r; hinduction s; hinduction q; hinduction p; reflexivity
 
   @[hott] def apdt02  {p q : x = y} (f : Π x, P x) (r : p = q) :
     apdt f p = transport2 P r (f x) ⬝ apdt f q :=
-  by induction r; exact !idp_con⁻¹
+  by hinduction r; exact !idp_con⁻¹
 
 end eq
 
