src/hott/init/pathover.lean
@@ -19,7 +19,7 @@ variables {A : Type _} {A' : Type _} {B : A → Type _} {B' : A → Type _} {B''
           {c : C b} {c₂ : C b₂}
 
 namespace eq
-  inductive pathover (B : A → Type.{l}) (b : B a) : Π{a₂ : A}, a = a₂ → B a₂ → Type.{l}
+  inductive pathover (B : A → Type l) (b : B a) : Π{a₂ : A}, a = a₂ → B a₂ → Type l
   | idpatho : pathover (refl a) b
 
   notation b ` =[`:50 p:0 `] `:0 b₂:50 := pathover _ b p b₂
@@ -34,25 +34,25 @@ namespace eq
 
   /- equivalences with equality using transport -/
   @[hott] def pathover_of_tr_eq (r : p ▸ b = b₂) : b =[p] b₂ :=
-  by induction p; induction r; constructor
+  by hinduction p; hinduction r; constructor
 
   @[hott] def pathover_of_eq_tr (r : b = p⁻¹ ▸ b₂) : b =[p] b₂ :=
-  begin induction p, change b = b₂ at r, induction r, constructor end
+  begin hinduction p, dsimp at r, hinduction r, constructor end
 
   @[hott] def tr_eq_of_pathover (r : b =[p] b₂) : p ▸ b = b₂ :=
-  by induction r; reflexivity
+  by hinduction r; reflexivity
 
   @[hott] def eq_tr_of_pathover (r : b =[p] b₂) : b = p⁻¹ ▸ b₂ :=
-  by induction r; reflexivity
+  by hinduction r; reflexivity
 
   @[hott] def pathover_equiv_tr_eq (p : a = a₂) (b : B a) (b₂ : B a₂)
     : (b =[p] b₂) ≃ (p ▸ b = b₂) :=
   begin
     fapply equiv.MK,
-    { exact tr_eq_of_pathover},
-    { exact pathover_of_tr_eq},
-    { intro r, induction p, induction r, apply idp},
-    { intro r, induction r, apply idp},
+    { exact tr_eq_of_pathover },
+    { exact pathover_of_tr_eq },
+    { intro r, hinduction p, hinduction r, refl },
+    { intro r, hinduction r, refl },
   end
 
   @[hott] def pathover_equiv_eq_tr (p : a = a₂) (b : B a) (b₂ : B a₂)
@@ -61,27 +61,27 @@ namespace eq
     fapply equiv.MK,
     { exact eq_tr_of_pathover},
     { exact pathover_of_eq_tr},
-    { intro r, induction p, change b = b₂ at r, induction r, apply idp},
-    { intro r, induction r, apply idp},
+    { intro r, hinduction p, change b = b₂ at r, hinduction r, apply idp},
+    { intro r, hinduction r, apply idp},
   end
 
   @[hott] def pathover_tr (p : a = a₂) (b : B a) : b =[p] p ▸ b :=
-  by induction p; constructor
+  by hinduction p; constructor
 
   @[hott] def tr_pathover (p : a = a₂) (b : B a₂) : p⁻¹ ▸ b =[p] b :=
-  by induction p; constructor
+  by hinduction p; constructor
 
   @[hott] def concato (r : b =[p] b₂) (r₂ : b₂ =[p₂] b₃) : b =[p ⬝ p₂] b₃ :=
-  by induction r₂; exact r
+  by hinduction r₂; exact r
 
   @[hott] def inverseo (r : b =[p] b₂) : b₂ =[p⁻¹] b :=
-  by induction r; constructor
+  by hinduction r; constructor
 
   @[hott] def concato_eq (r : b =[p] b₂) (q : b₂ = b₂') : b =[p] b₂' :=
-  by induction q; exact r
+  by hinduction q; exact r
 
   @[hott] def eq_concato (q : b = b') (r : b' =[p] b₂) : b =[p] b₂ :=
-  by induction q; exact r
+  by hinduction q; exact r
 
   @[hott] def change_path (q : p = p') (r : b =[p] b₂) : b =[p'] b₂ :=
   q ▸ r
@@ -117,41 +117,41 @@ namespace eq
   by refl
 
   @[hott] def idpo_cono (r : b =[p] b₂) : idpo ⬝o r =[idp_con p; λ x, b =[x] b₂] r :=
-  by induction r; refl
+  by hinduction r; refl
 
   @[hott] def cono.assoc' (r : b =[p] b₂) (r₂ : b₂ =[p₂] b₃) (r₃ : b₃ =[p₃] b₄) :
     r ⬝o (r₂ ⬝o r₃) =[con.assoc' _ _ _; λ x, b =[x] b₄] ((r ⬝o r₂) ⬝o r₃) :=
-  by induction r₃; induction r₂; induction r; refl
+  by hinduction r₃; hinduction r₂; hinduction r; refl
 
   @[hott] def cono.assoc (r : b =[p] b₂) (r₂ : b₂ =[p₂] b₃) (r₃ : b₃ =[p₃] b₄) :
     (r ⬝o r₂) ⬝o r₃ =[con.assoc _ _ _; λ x, b =[x] b₄] r ⬝o (r₂ ⬝o r₃) :=
-  by induction r₃; induction r₂; induction r; refl
+  by hinduction r₃; hinduction r₂; hinduction r; refl
 
   @[hott] def cono.right_inv (r : b =[p] b₂) : r ⬝o r⁻¹ᵒ =[con.right_inv _; λ x, b =[x] b] idpo :=
-  by induction r; refl
+  by hinduction r; refl
 
   @[hott] def cono.left_inv (r : b =[p] b₂) : r⁻¹ᵒ ⬝o r =[con.left_inv _; λ x, b₂ =[x] b₂] idpo :=
-  by induction r; refl
+  by hinduction r; refl
 
   @[hott] def eq_of_pathover {a' a₂' : A'} (q : a' =[p; λ _, A'] a₂') : a' = a₂' :=
-  by induction q; refl
+  by hinduction q; refl
 
   @[hott] def pathover_of_eq (p : a = a₂) {a' a₂' : A'} (q : a' = a₂') : a' =[p; λ _, A'] a₂' :=
-  by induction p; induction q; constructor
+  by hinduction p; hinduction q; constructor
 
   @[hott] def pathover_constant (p : a = a₂) (a' a₂' : A') : a' =[p; λ _, A'] a₂' ≃ a' = a₂' :=
   begin
     fapply equiv.MK,
     { exact eq_of_pathover},
     { exact pathover_of_eq p},
-    abstract { intro r, induction p, induction r, refl},
-    abstract { intro r, induction r, refl},
+    abstract { intro r, hinduction p, hinduction r, refl},
+    abstract { intro r, hinduction r, refl},
   end
 
   @[hott]
   def pathover_of_eq_tr_constant_inv (p : a = a₂) (a' : A')
     : pathover_of_eq p (tr_constant p a')⁻¹ = pathover_tr p a' :=
-  by induction p; constructor
+  by hinduction p; constructor
 
   @[hott, elab_simple]
   def eq_of_pathover_idp {b' : B a} (q : b =[idpath a] b') : b = b' :=
@@ -176,11 +176,11 @@ namespace eq
   @[hott, hsimp]
   def eq_of_pathover_idp_pathover_of_eq {A X : Type _} (x : X) {a a' : A} (p : a = a') :
     eq_of_pathover_idp (pathover_of_eq (idpath x) p) = p :=
-  by induction p; refl
+  by hinduction p; refl
 
   variable (B)
   @[hott, hsimp] def idpo_concato_eq (r : b = b') : eq_of_pathover_idp (@idpo A B a b ⬝op r) = r :=
-  by induction r; reflexivity
+  by hinduction r; reflexivity
   variable {B}
 
   -- def pathover_idp (b : B a) (b' : B a) : b =[idpath a] b' ≃ b = b' :=
@@ -192,8 +192,9 @@ namespace eq
   -- def pathover_idp_of_eq [reducible] {b' : B a} (q : b = b') : b =[idpath a] b' :=
   -- to_inv !pathover_idp q
 
-  @[hott, elab_as_eliminator, reducible, recursor] def idp_rec_on {P : Π⦃b₂ : B a⦄, b =[idpath a] b₂ → Sort u}
-    {b₂ : B a} (r : b =[idpath a] b₂) (H : P idpo) : P r :=
+  attribute [induction, priority 1000] pathover.rec 
+  @[hott, elab_as_eliminator, reducible, induction, priority 500] def idp_rec_on {P : Π⦃b₂ : B a⦄, b =[hott.eq.refl a] b₂ → Type u}
+    {b₂ : B a} (r : b =[hott.eq.refl a] b₂) (H : P idpo) : P r :=
   by exact
   have H2 : P (pathover_idp_of_eq B (eq_of_pathover_idp r)), from
     eq.rec_on (eq_of_pathover_idp r) H,
@@ -203,21 +204,20 @@ namespace eq
 
   @[hott] def rec_on_right {P : Π⦃b₂ : B a₂⦄, b =[p] b₂ → Type _}
     {b₂ : B a₂} (r : b =[p] b₂) (H : P (pathover_tr _ _)) : P r :=
-  by induction r; exact H
+  by hinduction r; exact H
 
   @[hott] def rec_on_left {P : Π⦃b : B a⦄, b =[p] b₂ → Type _}
     {b : B a} (r : b =[p] b₂) (H : P (tr_pathover _ _)) : P r :=
-  by induction r; exact H
+  by hinduction r; exact H
 
-  --pathover with fibration B' ∘ f
   @[hott] def pathover_ap (B' : A' → Type _) (f : A → A') {p : a = a₂}
     {b : B' (f a)} {b₂ : B' (f a₂)} (q : b =[p; B' ∘ f] b₂) : b =[ap f p] b₂ :=
-  by induction q; constructor
+  by hinduction q; constructor
 
   @[hott] def pathover_of_pathover_ap (B' : A' → Type u) (f : A → A') {p : a = a₂}
     {b : B' (f a)} {b₂ : B' (f a₂)} (q : b =[ap f p] b₂) : b =[p; B' ∘ f] b₂ :=
   begin
-    induction p, induction q using hott.eq.idp_rec_on, exact idpo
+    hinduction p, hinduction q, exact idpo
   end
 
   @[hott] def pathover_compose (B' : A' → Type _) (f : A → A') (p : a = a₂)
@@ -226,8 +226,8 @@ namespace eq
     fapply equiv.MK,
     { exact pathover_ap B' f},
     { exact pathover_of_pathover_ap B' f},
-    { intro q, induction p, induction q using hott.eq.idp_rec_on, refl},
-    { intro q, induction q, refl},
+    { intro q, hinduction p, hinduction q, refl},
+    { intro q, hinduction q, refl},
   end
 
   @[hott] def pathover_of_pathover_tr (q : b =[p ⬝ p₂] p₂ ▸ b₂) : b =[p] b₂ :=
@@ -243,10 +243,10 @@ namespace eq
   pathover_cancel_left (pathover_tr _ _)⁻¹ᵒ q
 
   @[hott] def pathover_tr_of_eq (q : b = b') : b =[p] p ▸ b' :=
-  by induction q;apply pathover_tr
+  by hinduction q;apply pathover_tr
 
   @[hott] def tr_pathover_of_eq (q : b₂ = b₂') : p⁻¹ ▸ b₂ =[p] b₂' :=
-  by induction q;apply tr_pathover
+  by hinduction q;apply tr_pathover
 
   @[hott] def eq_of_parallel_po_right (q : b =[p] b₂) (q' : b =[p] b₂') : b₂ = b₂' :=
   begin
@@ -262,74 +262,73 @@ namespace eq
 
   variable (C)
   @[hott, elab_simple] def transporto (r : b =[p] b₂) (c : C b) : C b₂ :=
-  by induction r;exact c
+  by hinduction r;exact c
   infix ` ▸o `:75 := transporto _
 
   @[hott] def fn_tro_eq_tro_fn {C' : Π ⦃a : A⦄, B a → Type _} (q : b =[p] b₂)
     (f : Π⦃a : A⦄ (b : B a), C b → C' b) (c : C b) : f b₂ (q ▸o c) = q ▸o (f b c) :=
-  by induction q; reflexivity
+  by hinduction q; reflexivity
   variable {C}
 
   /- various variants of ap for pathovers -/
   @[hott] def apd (f : Πa, B a) (p : a = a₂) : f a =[p] f a₂ :=
-  by induction p; constructor
+  by hinduction p; constructor
 
   @[hott] def apd_idp (f : Πa, B a) : apd f idp = @idpo A B a (f a) :=
   by reflexivity
 
   @[hott] def apo {f : A → A'} (g : Πa, B a → B'' (f a)) (q : b =[p] b₂) :
     g a b =[p; B'' ∘ f] g a₂ b₂ :=
-  by induction q; constructor
+  by hinduction q; constructor
 
   @[hott] def apd011 (f : Πa, B a → A') (Ha : a = a₂) (Hb : b =[Ha] b₂)
       : f a b = f a₂ b₂ :=
-  by induction Hb; reflexivity
+  by hinduction Hb; reflexivity
 
   @[hott] def apd0111 (f : Πa b, C b → A') (Ha : a = a₂) (Hb : b =[Ha] b₂)
     (Hc : c =[apd011 C Ha Hb; id] c₂) : f a b c = f a₂ b₂ c₂ :=
-  by induction Hb; induction Hc using hott.eq.idp_rec_on; refl
+  begin hinduction Hb, hinduction Hc, refl end
 
   @[hott] def apod11 {f : Πb, C b} {g : Πb₂, C b₂} (r : f =[p; λ a, Π b : B a, C b] g)
     {b : B a} {b₂ : B a₂} (q : b =[p] b₂) : f b =[apd011 C p q; id] g b₂ :=
-  by induction r; induction q using hott.eq.idp_rec_on; constructor
+  by hinduction r; hinduction q; constructor
 
   @[hott] def apdo10 {f : Πb, C b} {g : Πb₂, C b₂} (r : f =[p; λ a, Π b : B a, C b] g)
     (b : B a) : f b =[apd011 C p (pathover_tr _ _); id] g (p ▸ b) :=
-  by induction r; constructor
+  by hinduction r; constructor
 
   @[hott] def apo10 {f : B a → B' a} {g : B a₂ → B' a₂} (r : f =[p; λ a, B a → B' a] g)
     (b : B a) : f b =[p] g (p ▸ b) :=
-  by induction r; constructor
+  by hinduction r; constructor
 
   @[hott] def apo10_constant_right {f : B a → A'} {g : B a₂ → A'} (r : f =[p; λ a, B a → A'] g)
     (b : B a) : f b = g (p ▸ b) :=
-  by induction r; constructor
+  by hinduction r; constructor
 
   @[hott] def apo10_constant_left {f : A' → B a} {g : A' → B a₂} (r : f =[p; λ a, A' → B a] g)
     (a' : A') : f a' =[p] g a' :=
-  by induction r; constructor
+  by hinduction r; constructor
 
   @[hott] def apo11 {f : B a → B' a} {g : B a₂ → B' a₂} (r : f =[p; λ a, B a → B' a] g)
     (q : b =[p] b₂) : f b =[p] g b₂ :=
-  by induction q; exact apo10 r b
+  by hinduction q; exact apo10 r b
 
   @[hott] def apo011 {A : Type _} {B C D : A → Type _} {a a' : A} {p : a = a'} {b : B a} {b' : B a'}
     {c : C a} {c' : C a'} (f : Π⦃a⦄, B a → C a → D a) (q : b =[p] b') (r : c =[p] c') :
     f b c =[p] f b' c' :=
-  begin induction q, induction r using hott.eq.idp_rec_on, exact idpo end
+  begin hinduction q, hinduction r, exact idpo end
 
   @[hott] def apdo011 {A : Type _} {B : A → Type _} {C : Π⦃a⦄, B a → Type _}
     (f : Π⦃a⦄ (b : B a), C b) {a a' : A} (p : a = a') {b : B a} {b' : B a'} (q : b =[p] b')
       : f b =[apd011 C p q; id] f b' :=
-  by induction q; constructor
+  by hinduction q; constructor
 
   @[hott] def apdo0111 {A : Type _} {B : A → Type _} {C C' : Π⦃a⦄, B a → Type _}
     (f : Π⦃a⦄ {b : B a}, C b → C' b) {a a' : A} (p : a = a') {b : B a} {b' : B a'} (q : b =[p] b')
     {c : C b} {c' : C b'} (r : c =[apd011 C p q; id] c')
       : f c =[apd011 C' p q; id] f c' :=
   begin
-    induction q, dsimp [apd011] at r,
-    induction r using hott.eq.idp_rec_on, refl
+    hinduction q, hinduction r, refl
   end
 
   @[hott] def apo11_constant_right {f : B a → A'} {g : B a₂ → A'}
@@ -339,10 +338,10 @@ namespace eq
   /- properties about these "ap"s, transporto and pathover_ap -/
   @[hott] def apd_con (f : Πa, B a) (p : a = a₂) (q : a₂ = a₃)
     : apd f (p ⬝ q) = apd f p ⬝o apd f q :=
-  by induction p; induction q; reflexivity
+  by hinduction p; hinduction q; reflexivity
 
   @[hott] def apd_inv (f : Πa, B a) (p : a = a₂) : apd f p⁻¹ = (apd f p)⁻¹ᵒ :=
-  by induction p; reflexivity
+  by hinduction p; reflexivity
 
   @[hott] def apd_eq_pathover_of_eq_ap (f : A → A') (p : a = a₂) :
     apd f p = pathover_of_eq p (ap f p) :=
@@ -350,60 +349,60 @@ namespace eq
 
   @[hott] def apo_invo (f : Πa, B a → B' a) {Ha : a = a₂} (Hb : b =[Ha] b₂)
       : (apo f Hb)⁻¹ᵒ = apo f Hb⁻¹ᵒ :=
-  by induction Hb; reflexivity
+  by hinduction Hb; reflexivity
 
   @[hott] def apd011_inv (f : Πa, B a → A') (Ha : a = a₂) (Hb : b =[Ha] b₂)
       : (apd011 f Ha Hb)⁻¹ = (apd011 f Ha⁻¹ Hb⁻¹ᵒ) :=
-  by induction Hb; reflexivity
+  by hinduction Hb; reflexivity
 
   @[hott] def cast_apd011 (q : b =[p] b₂) (c : C b) : cast (apd011 C p q) c = q ▸o c :=
-  by induction q; reflexivity
+  by hinduction q; reflexivity
 
   @[hott] def apd_compose1 (g : Πa, B a → B' a) (f : Πa, B a) (p : a = a₂)
     : apd (g ∘' f) p = apo g (apd f p) :=
-  by induction p; reflexivity
+  by hinduction p; reflexivity
 
   @[hott] def apd_compose2 (g : Πa', B'' a') (f : A → A') (p : a = a₂)
     : apd (λa, g (f a)) p = pathover_of_pathover_ap B'' f (apd g (ap f p)) :=
-  by induction p; reflexivity
+  by hinduction p; reflexivity
 
   @[hott] def apo_tro (C : Π⦃a⦄, B' a → Type _) (f : Π⦃a⦄, B a → B' a) (q : b =[p] b₂)
     (c : C (f b)) : apo f q ▸o c = q ▸o c :=
-  by induction q; reflexivity
+  by hinduction q; reflexivity
 
   @[hott] def pathover_ap_tro {B' : A' → Type _} (C : Π⦃a'⦄, B' a' → Type _) (f : A → A')
     {b : B' (f a)} {b₂ : B' (f a₂)} (q : b =[p; B' ∘ f] b₂) (c : C b) :
     pathover_ap B' f q ▸o c = q ▸o c :=
-  by induction q; reflexivity
+  by hinduction q; reflexivity
 
   @[hott] def pathover_ap_invo_tro {B' : A' → Type _} (C : Π⦃a'⦄, B' a' → Type _) (f : A → A')
     {b : B' (f a)} {b₂ : B' (f a₂)} (q : b =[p; B' ∘ f] b₂) (c : C b₂)
     : (pathover_ap B' f q)⁻¹ᵒ ▸o c = q⁻¹ᵒ ▸o c :=
-  by induction q; reflexivity
+  by hinduction q; reflexivity
 
   @[hott, elab_simple] def pathover_tro (q : b =[p] b₂) (c : C b) : c =[apd011 C p q; id] q ▸o c :=
-  by induction q; constructor
+  by hinduction q; constructor
 
   @[hott] def pathover_ap_invo {B' : A' → Type _} (f : A → A') {p : a = a₂}
     {b : B' (f a)} {b₂ : B' (f a₂)} (q : b =[p; B' ∘ f] b₂)
     : pathover_ap B' f q⁻¹ᵒ =[ap_inv f p; λ x, b₂ =[x] b] (pathover_ap B' f q)⁻¹ᵒ :=
-  by induction q; exact idpo
+  by hinduction q; exact idpo
 
   @[hott] def tro_invo_tro {A : Type _} {B : A → Type _} (C : Π⦃a⦄, B a → Type _)
     {a a' : A} {p : a = a'} {b : B a} {b' : B a'} (q : b =[p] b') (c : C b') :
     q ▸o (q⁻¹ᵒ ▸o c) = c :=
-  by induction q; reflexivity
+  by hinduction q; reflexivity
 
   @[hott] def invo_tro_tro {A : Type _} {B : A → Type _} (C : Π⦃a⦄, B a → Type _)
     {a a' : A} {p : a = a'} {b : B a} {b' : B a'} (q : b =[p] b') (c : C b) :
     q⁻¹ᵒ ▸o (q ▸o c) = c :=
-  by induction q; reflexivity
+  by hinduction q; reflexivity
 
   @[hott] def cono_tro {A : Type _} {B : A → Type _} (C : Π⦃a⦄, B a → Type _)
     {a₁ a₂ a₃ : A} {p₁ : a₁ = a₂} {p₂ : a₂ = a₃} {b₁ : B a₁} {b₂ : B a₂} {b₃ : B a₃}
     (q₁ : b₁ =[p₁] b₂) (q₂ : b₂ =[p₂] b₃) (c : C b₁) :
     transporto C (q₁ ⬝o q₂) c = transporto C q₂ (transporto C q₁ c) :=
-  by induction q₂; reflexivity
+  by hinduction q₂; reflexivity
 
   @[hott] def is_equiv_transporto {A : Type _} {B : A → Type _} (C : Π⦃a⦄, B a → Type _)
     {a a' : A} {p : a = a'} {b : B a} {b' : B a'} (q : b =[p] b') : is_equiv (transporto C q) :=
@@ -422,19 +421,19 @@ namespace eq
 
   @[hott] def cono.right_inv_eq (q : b = b') :
     pathover_idp_of_eq B q ⬝op q⁻¹ = (idpo : b =[refl a] b) :=
-  by induction q;constructor
+  by hinduction q;constructor
 
   @[hott] def cono.right_inv_eq' (q : b = b') :
     q ⬝po (pathover_idp_of_eq B q⁻¹) = (idpo : b =[refl a] b) :=
-  by induction q;constructor
+  by hinduction q;constructor
 
   @[hott] def cono.left_inv_eq (q : b = b') :
     pathover_idp_of_eq B q⁻¹ ⬝op q = (idpo : b' =[refl a] b') :=
-  by induction q;constructor
+  by hinduction q;constructor
 
   @[hott] def cono.left_inv_eq' (q : b = b') :
     q⁻¹ ⬝po pathover_idp_of_eq B q = (idpo : b' =[refl a] b') :=
-  by induction q;constructor
+  by hinduction q;constructor
 
   @[hott] def pathover_of_fn_pathover_fn (f : Π{a}, B a ≃ B' a) (r : f.to_fun b =[p] f.to_fun b₂) : b =[p] b₂ :=
   (left_inv f.to_fun b)⁻¹ ⬝po apo (λa, to_fun f⁻¹ᵉ) r ⬝op left_inv f.to_fun b₂
@@ -443,11 +442,11 @@ namespace eq
     an equality with a change_path -/
   @[hott] def change_path_of_pathover (s : p = p') (r : b =[p] b₂) (r' : b =[p'] b₂)
     (q : r =[s; λ p, b =[p] b₂] r') : change_path s r = r' :=
-  by induction s; induction q using hott.eq.idp_rec_on; reflexivity
+  by hinduction s; hinduction q; reflexivity
 
   @[hott] def pathover_of_change_path (s : p = p') (r : b =[p] b₂) (r' : b =[p'] b₂)
     (q : change_path s r = r') : r =[s; λ p, b =[p] b₂] r' :=
-  by induction s; induction q; constructor
+  by hinduction s; hinduction q; constructor
 
   @[hott] def pathover_pathover_path (s : p = p') (r : b =[p] b₂) (r' : b =[p'] b₂) :
     (r =[s; λ p, b =[p] b₂] r') ≃ change_path s r = r' :=
@@ -455,17 +454,17 @@ namespace eq
     fapply equiv.MK,
     { apply change_path_of_pathover},
     { apply pathover_of_change_path},
-    { intro q, induction s, induction q, reflexivity},
-    { intro q, induction s, induction q using hott.eq.idp_rec_on, reflexivity},
+    { intro q, hinduction s, hinduction q, reflexivity},
+    { intro q, hinduction s, hinduction q, reflexivity},
   end
 
   /- variants of inverse2 and concat2 -/
   @[hott] def inverseo2 {r r' : b =[p] b₂} (s : r = r') : r⁻¹ᵒ = r'⁻¹ᵒ :=
-  by induction s; reflexivity
+  by hinduction s; reflexivity
 
   @[hott] def concato2 {r r' : b =[p] b₂} {r₂ r₂' : b₂ =[p₂] b₃}
     (s : r = r') (s₂ : r₂ = r₂') : r ⬝o r₂ = r' ⬝o r₂' :=
-  by induction s; induction s₂; reflexivity
+  by hinduction s; hinduction s₂; reflexivity
 
   infixl ` ◾o `:75 := concato2
   postfix [parsing_only] `⁻²ᵒ`:(max+10) := inverseo2 --this notation is abusive, should we use it?
@@ -475,7 +474,7 @@ namespace eq
     {k : A → A} {l : Π⦃a⦄, B a → B (k a)} (m : Π⦃a⦄ {b : B a}, C b → C (l b))
     (c : C b) :
     m (q ▸o c) = (pathover_ap B k (apo l q)) ▸o (m c) :=
-  by induction q; reflexivity
+  by hinduction q; reflexivity
 
   @[hott] def apd0111_precompose (f : Π⦃a⦄ {b : B a}, C b → A')
     {k : A → A} {l : Π⦃a⦄, B a → B (k a)} (m : Π⦃a⦄ {b : B a}, C b → C (l b))
@@ -483,7 +482,7 @@ namespace eq
     : @apd0111 _ _ B _ _ _ _ _ _ _  (λa b (c : C b), f (m c)) p q (pathover_tro q c) ⬝
         ap (@f _ _) (fn_tro_eq_tro_fn2 q m c) =
       apd0111 f (ap k p) (pathover_ap B k (apo l q)) (pathover_tro _ (m c)) :=
-  by induction q; reflexivity
+  by hinduction q; reflexivity
 
 end eq
 
